prep fib (use Racket to generate += expressions and move pow into util)

rkt/fib_rec.rkt
@@ -1,0 +1,16 @@
+#lang at-exp s-exp "tmonad.rkt"
+
+(Fixpoint
+ fib_rec @n{nat} 
+  #:returns @{nat}
+ (match (n)
+   [0 => (<== 1)]
+   [(S n′) 
+    => 
+    (match (n′)
+      [0 => (<== 1)]
+      [(S n′′)
+       =>
+       (bind ((a (fib_rec n′′)))
+             (bind ((b (fib_rec n′)))
+                   (<== (+ a b))))])]))
