common/pow.v
@@ -1,0 +1,28 @@
+Require Import Arith Arith.Even Arith.Div2 Omega.
+Require Import Coq.Logic.JMeq Coq.Program.Wf.
+Require Import Program.Syntax List.
+Require Import Braun.common.util.
+
+Fixpoint pow n m :=
+  match m with
+    | O =>
+      1
+    | S m =>
+      n + pow n m
+  end.
+
+Lemma pow2_monotone:
+  forall x y,
+    x <= y ->
+    pow 2 x <= pow 2 y.
+Proof.
+  induction x as [|x]; intros y LE.
+  simpl.
+  destruct y as [|y]. simpl. auto.
+  simpl. omega.
+  destruct y as [|y]. omega.
+  apply le_S_n in LE.
+  apply IHx in LE.
+  simpl.  omega.
+Qed.
+  
